drop ext_map and further progress

src/theory/bir/bir_envScript.sml
@@ -5,18 +5,6 @@ open bir_auxiliaryTheory bir_immTheory bir_valuesTheory;
 
 val _ = new_theory "bir_env";
 
-val _ = Datatype `bir_ext_map_t = BExtMap (string |-> ('ext_state_t -> bir_val_t option)) (string |-> (bir_val_t -> 'ext_state_t -> 'ext_state_t option))`;
-
-val bir_lookup_get_def = Define `
-  bir_lookup_get ((BExtMap get_map put_map):'ext_state_t bir_ext_map_t) ext_name =
-    FLOOKUP get_map ext_name
-`;
-
-val bir_lookup_put_def = Define `
-  bir_lookup_put ((BExtMap get_map put_map):'ext_state_t bir_ext_map_t) ext_name =
-    FLOOKUP put_map ext_name
-`;
-
 val _ = Datatype `bir_var_t = BVar string bir_type_t`;
 
 val bir_var_name_def = Define `bir_var_name (BVar n _) = n`;
@@ -351,102 +339,23 @@ val bir_envty_includes_vs_SUBSET = store_thm("bir_envty_includes_vs_SUBSET", ``
 
 (* ===================== *)
 
-val _ = Datatype `bir_var_ext_env_typing_t = BExtEnvTy (string -> (bir_type_t option))`;
-
-val bir_ext_envty_of_ext_env_def = Define `bir_ext_envty_of_ext_env ((BExtMap ext_get_map ext_put_map):'ext_state_t bir_ext_map_t, ext_st) =
-  BExtEnvTy (( \ f. OPTION_BIND f ( \ f'. OPTION_MAP type_of_bir_val (f' ext_st))) o (FLOOKUP ext_get_map))
-`;
-
-(* Note that this is only defined for get functions, for now... *)
-val bir_ext_env_satisfies_ext_envty_def = Define `
-  bir_ext_env_satisfies_ext_envty (ext_map, ext_st:'ext_state_t) (BExtEnvTy ext_envty) <=>
-    !ext_name ty.
-      ext_envty ext_name = SOME ty ==>
-      ?f_get v. bir_lookup_get ext_map ext_name = SOME f_get /\
-          f_get ext_st = SOME v /\ type_of_bir_val v = ty`;
-
-val bir_ext_env_satisfies_ext_envty_of_ext_env = store_thm("bir_ext_env_satisfies_ext_envty_of_ext_env", ``
-  !ext_map (ext_st:'ext_state_t). bir_ext_env_satisfies_ext_envty (ext_map, ext_st) (bir_ext_envty_of_ext_env (ext_map, ext_st))
-``,
-  Cases_on `ext_map` >>
-  SIMP_TAC std_ss [bir_ext_env_satisfies_ext_envty_def, bir_ext_envty_of_ext_env_def, bir_lookup_get_def] >>
-  rpt strip_tac >>
-  metis_tac[]
-);
-
-val bir_ext_envty_includes_ext_def = Define `
-  bir_ext_envty_includes_ext (BExtEnvTy ext_envty) (ext_name, ext_ty) <=>
-  ext_envty ext_name = SOME ext_ty`;
-
-val bir_ext_envty_includes_exts_def = Define `
-  (bir_ext_envty_includes_exts ext_envty exts =
-  !ext. ext IN exts ==> bir_ext_envty_includes_ext ext_envty ext)`;
-
-val bir_eval_extget_def = Define `
-  (bir_eval_extget (ext_map:'ext_state_t bir_ext_map_t) ext_name ty ext_st =
-    case bir_lookup_get ext_map ext_name of
-    | SOME f_get =>
-      (case f_get ext_st of
+Definition bir_eval_extget_def:
+  bir_eval_extget ext_fn ty ext_st =
+      case ext_fn ext_st of
        | SOME v =>
         if type_of_bir_val v <> ty
         then NONE
         else SOME v
-       | NONE => NONE)
-    | NONE => NONE)`;
+       | NONE => NONE
+End
 
-val bir_eval_extget_type = store_thm ("bir_eval_extget_type",
-``!ext_map (ext_st:'ext_state_t) ext_name ext_ty v.
-  bir_eval_extget ext_map ext_name ext_ty ext_st = SOME v ==>
-  type_of_bir_val v = ext_ty``,
-
-  rpt strip_tac >>
-  fs[bir_eval_extget_def] >>
-  Cases_on `bir_lookup_get ext_map ext_name` >> (
-    fs[]
-  ) >>
-  Cases_on `x ext_st` >> (
-    gvs[]
-  )
-);
-
-val bir_ext_in_ext_envty_ext_env_IMP = store_thm ("bir_ext_in_ext_envty_ext_env_IMP",
-``!ext_envty ext_map (ext_st:'ext_state_t) ext_name ext_ty.
-        bir_ext_envty_includes_ext ext_envty (ext_name, ext_ty) ==>
-        bir_ext_env_satisfies_ext_envty (ext_map, ext_st) ext_envty ==>
-        ?va.
-          bir_eval_extget ext_map ext_name ext_ty ext_st = SOME va /\ type_of_bir_val va = ext_ty``,
-
-  rpt strip_tac >>
-  Cases_on `ext_envty` >>
-  fs[bir_ext_envty_includes_ext_def, bir_ext_env_satisfies_ext_envty_def, bir_eval_extget_def] >>
-  RES_TAC >>
-  fs[]
-);
-
-val bir_ext_envty_includes_exts_EMPTY = store_thm("bir_ext_envty_includes_exts_EMPTY", ``
-  !ext_envty. (bir_ext_envty_includes_exts ext_envty EMPTY)
-``,
-  Cases_on `ext_envty` >>
-  SIMP_TAC std_ss [bir_ext_envty_includes_exts_def, bir_ext_envty_includes_ext_def, NOT_IN_EMPTY]
-);
-
-val bir_ext_envty_includes_exts_INSERT = store_thm("bir_ext_envty_includes_exts_INSERT", ``
-  !ext_envty ext exts. (bir_ext_envty_includes_exts ext_envty (ext INSERT exts)) <=>
-               ((bir_ext_envty_includes_ext ext_envty ext) /\ (bir_ext_envty_includes_exts ext_envty exts))
-``,
-  Cases_on `ext_envty` >>
-  SIMP_TAC std_ss [bir_ext_envty_includes_exts_def, IN_INSERT] >>
-  METIS_TAC[]
-);
-
-val bir_ext_envty_includes_exts_UNION = store_thm("bir_ext_envty_includes_exts_UNION", ``
-  !ext_envty exts1 exts2. (bir_ext_envty_includes_exts ext_envty (exts1 UNION exts2)) <=>
-                  ((bir_ext_envty_includes_exts ext_envty exts1) /\ (bir_ext_envty_includes_exts ext_envty exts2))
-``,
-  Cases_on `ext_envty` >>
-  SIMP_TAC std_ss [bir_ext_envty_includes_exts_def, IN_UNION] >>
-  METIS_TAC[]
-);
+Theorem bir_eval_extget_type:
+  !ext_st ext_fn ext_ty v.
+  bir_eval_extget ext_fn ext_ty ext_st = SOME v ==>
+  type_of_bir_val v = ext_ty
+Proof
+  rpt strip_tac >> fs[bir_eval_extget_def,AllCaseEqs()]
+QED
 
 (* ===================== *)
 
