src/theory/bir-support/bir_program_varsScript.sml
@@ -198,7 +198,6 @@ val bir_state_EQ_FOR_VARS_ALT_DEF = store_thm ("bir_state_EQ_FOR_VARS_ALT_DEF",
 ``!vs st1 st2.
   bir_state_EQ_FOR_VARS vs st1 st2 <=>
   (st1.bst_pc = st2.bst_pc) /\ (st1.bst_status = st2.bst_status) /\
-  (st1.bst_inflight = st2.bst_inflight) /\ (st1.bst_counter = st2.bst_counter) /\
   (st1.bst_viewenv = st2.bst_viewenv) /\ (st1.bst_v_rOld = st2.bst_v_rOld) /\
   (st1.bst_v_CAP = st2.bst_v_CAP) /\ (st1.bst_v_Rel = st2.bst_v_Rel) /\
   (st1.bst_v_rNew = st2.bst_v_rNew) /\ (st1.bst_v_wNew = st2.bst_v_wNew) /\
