src/theory/bir/bir_env_oldScript.sml
@@ -81,49 +81,6 @@ val bir_env_vars_are_initialised_EQ_envty = store_thm("bir_env_vars_are_initiali
 
 (* ===================== *)
 
-val bir_ext_env_ext_is_valid_def = Define `
-  (bir_ext_env_ext_is_valid (ext_map, ext_st:'ext_state_t) (ext_name, ext_ty) <=>
-  (?v. (bir_eval_extget ext_map ext_name ext_ty ext_st = SOME v) /\
-       (type_of_bir_val v = ext_ty)))`;
-
-val bir_ext_env_ext_is_valid_EQ_ext_envty = store_thm("bir_ext_env_ext_is_valid_EQ_ext_envty", ``
-  !(ext_map:'ext_state_t bir_ext_map_t) ext_st ext. bir_ext_env_ext_is_valid (ext_map, ext_st) ext <=> bir_ext_envty_includes_ext (bir_ext_envty_of_ext_env (ext_map, ext_st)) ext
-``,
-  Cases_on `ext_map` >> Cases_on `ext` >>
-  REWRITE_TAC [bir_ext_envty_of_ext_env_def, bir_ext_env_ext_is_valid_def, bir_ext_envty_includes_ext_def, bir_eval_extget_def] >>
-  SIMP_TAC std_ss [bir_lookup_get_def] >>
-  rpt strip_tac >>
-  Cases_on `FLOOKUP f q` >- (
-    fs[]
-  ) >>
-  fs[] >>
-  rpt strip_tac >>
-  eq_tac >> (
-    rpt strip_tac
-  ) >- (
-    Cases_on `x ext_st` >> (
-      fs[]
-    )
-  ) >>
-  Cases_on `x ext_st` >> (
-    fs[]
-  )
-);
-
-val bir_ext_env_exts_are_valid_def = Define `
-  bir_ext_env_exts_are_valid (ext_map, ext_st:'ext_state_t) exts <=>
-  (!ext. ext IN exts ==> bir_ext_env_ext_is_valid (ext_map, ext_st) ext)`;
-
-
-val bir_ext_env_exts_are_valid_EQ_ext_envty = store_thm("bir_ext_env_exts_are_valid_EQ_ext_envty", ``
-  !ext_env exts. bir_ext_env_exts_are_valid ext_env exts <=> bir_ext_envty_includes_exts (bir_ext_envty_of_ext_env ext_env) exts
-``,
-  Cases_on `ext_env` >>
-  REWRITE_TAC [bir_ext_env_exts_are_valid_def, bir_ext_envty_includes_exts_def, bir_ext_env_ext_is_valid_EQ_ext_envty]
-);
-
-(* ===================== *)
-
 val bir_env_var_is_initialised_weaken = store_thm ("bir_env_var_is_initialised_weaken",
   ``!v env. bir_env_var_is_initialised env v ==> bir_env_var_is_declared env v``,
 Cases >> SIMP_TAC std_ss [bir_env_var_is_initialised_def, bir_env_var_is_declared_def,
@@ -277,18 +234,6 @@ val bir_env_order_well_typed = store_thm ("bir_env_order_well_typed",
 REWRITE_TAC [bir_is_well_typed_env_THM]
 );
 
-
-(* ===================== *)
-
-val bir_ext_env_exts_are_valid_EMPTY = store_thm ("bir_ext_env_exts_are_valid_EMPTY",
-  ``!ext_map ext_st:'ext_state_t. bir_ext_env_exts_are_valid (ext_map, ext_st) {}``,
-SIMP_TAC std_ss [bir_ext_env_exts_are_valid_EQ_ext_envty, bir_ext_envty_includes_exts_EMPTY]);
-
-val bir_ext_env_exts_are_valid_UNION = store_thm ("bir_ext_env_exts_are_valid_UNION",
-  ``!ext_map ext_st:'ext_state_t exts1 exts2. bir_ext_env_exts_are_valid (ext_map, ext_st) (exts1 UNION exts2) <=>
-                  (bir_ext_env_exts_are_valid (ext_map, ext_st) exts1 /\
-                   bir_ext_env_exts_are_valid (ext_map, ext_st) exts2) ``,
-SIMP_TAC std_ss [bir_ext_env_exts_are_valid_EQ_ext_envty, bir_ext_env_ext_is_valid_EQ_ext_envty, bir_ext_envty_includes_exts_UNION]);
 
 (* ===================== *)
 
