src/theory/bir/bir_programScript.sml
@@ -22,7 +22,7 @@ val _ = Datatype `bir_label_t =
 
 val _ = Datatype `bir_label_exp_t =
     BLE_Label bir_label_t
-  | BLE_Exp bir_exp_t
+  | BLE_Exp ('ext_state_t bir_exp_t)
 `;
 
 val _ = Datatype `bir_memop_t =
@@ -39,43 +39,43 @@ val _ = Datatype `bir_memop_t =
 *)
 Datatype:
   bir_stmt_basic_t =
-  | BStmt_Assign bir_var_t bir_exp_t
-  | BStmt_Assert bir_exp_t
-  | BStmt_Assume bir_exp_t
+  | BStmt_Assign bir_var_t ('ext_state_t bir_exp_t)
+  | BStmt_Assert ('ext_state_t bir_exp_t)
+  | BStmt_Assume ('ext_state_t bir_exp_t)
 (*  | BStmt_ExtPut string bir_exp_t (* string should be looked up as a (bir_val_t -> 'ext_state_t -> 'ext_state_t option) *) *)
 End
 
 Datatype:
   bmc_stmt_basic_t =
   (* reg, address, cast, xcl, acq rel *)
-  | BMCStmt_Load bir_var_t bir_exp_t ((bir_cast_t # bir_immtype_t) option) bool bool bool
+  | BMCStmt_Load bir_var_t ('ext_state_t bir_exp_t) ((bir_cast_t # bir_immtype_t) option) bool bool bool
   (* success reg, address, value, xcl, acq, rel *)
-  | BMCStmt_Store bir_var_t bir_exp_t bir_exp_t bool bool bool
+  | BMCStmt_Store bir_var_t ('ext_state_t bir_exp_t) ('ext_state_t bir_exp_t) bool bool bool
   (* success reg, address, value, acq, rel *)
-  | BMCStmt_Amo bir_var_t bir_exp_t bir_exp_t bool bool
-  | BMCStmt_Assign bir_var_t bir_exp_t
+  | BMCStmt_Amo bir_var_t ('ext_state_t bir_exp_t) ('ext_state_t bir_exp_t) bool bool
+  | BMCStmt_Assign bir_var_t ('ext_state_t bir_exp_t)
   | BMCStmt_Fence bir_memop_t bir_memop_t
   (* TODO: Should take view of the input *)
-(*  | BMCStmt_ExtPut string bir_exp_t *)
-  | BMCStmt_Assert bir_exp_t
-  | BMCStmt_Assume bir_exp_t
+(*  | BMCStmt_ExtPut string ('ext_state_t bir_exp_t) *)
+  | BMCStmt_Assert ('ext_state_t bir_exp_t)
+  | BMCStmt_Assume ('ext_state_t bir_exp_t)
 End
 
 Datatype:
   bir_stmt_end_t =
-  | BStmt_Jmp     bir_label_exp_t
-  | BStmt_CJmp    bir_exp_t bir_label_exp_t bir_label_exp_t
-  | BStmt_Halt    bir_exp_t
+  | BStmt_Jmp     ('ext_state_t bir_label_exp_t)
+  | BStmt_CJmp    ('ext_state_t bir_exp_t) ('ext_state_t bir_label_exp_t) ('ext_state_t bir_label_exp_t)
+  | BStmt_Halt    ('ext_state_t bir_exp_t)
 End
 
 Datatype:
   bir_generic_stmt_t =
   | BStmtB 'a
-  | BStmtE bir_stmt_end_t
+  | BStmtE ('ext_state_t bir_stmt_end_t)
 End
 
-Type bir_stmt_t = ``:bir_stmt_basic_t bir_generic_stmt_t``
-Type bmc_stmt_t = ``:bmc_stmt_basic_t bir_generic_stmt_t``
+Type bir_stmt_t = ``:('ext_state_t bir_stmt_basic_t,'ext_state_t) bir_generic_stmt_t``
+Type bmc_stmt_t = ``:('ext_state_t bmc_stmt_basic_t,'ext_state_t) bir_generic_stmt_t``
 
 val _ = Datatype `bir_mc_tags_t = <|
   mc_acq            : bool;
@@ -95,19 +95,18 @@ val _ = Datatype `bir_status_t =
   | BST_Halted bir_val_t        (* Halt called *)
   | BST_JumpOutside bir_label_t (* Jump to unknown label *)`;
 
-val _ = Datatype `bir_inflight_stmt_t = BirInflight string bir_stmt_t`;
-
 (* forward buffer, part of the core-local state *)
-val fwdb_def = Datatype`
+Datatype:
   fwdb_t = <| fwdb_time : num; fwdb_view : num; fwdb_xcl : bool |>
-`;
+End
 
 (* exclusives bank, part of the core-local state *)
-val xclb_def = Datatype`
+Datatype:
   xclb_t = <| xclb_time : num; xclb_view : num |>
-`;
+End
 
-val _ = Datatype `bir_state_t = <|
+Datatype:
+  bir_state_t = <|
   bst_pc       : bir_programcounter_t;
   bst_environ  : bir_var_environment_t;
   bst_status   : bir_status_t;
@@ -122,52 +121,50 @@ val _ = Datatype `bir_state_t = <|
   bst_prom     : num list;
   bst_fwdb     : bir_val_t -> fwdb_t;
   bst_xclb     : xclb_t option;
-  bst_inflight : bir_inflight_stmt_t list;
-  bst_counter  : num
-|>`;
+|>
+End
+
+Type beb_relation_t =
+  ``: (bir_state_t # (bir_state_t -> bool) # 'ext_state_t)
+    -> (bir_state_t # 'ext_state_t) -> bool``
 
 val _ = Datatype `bir_generic_stmt_block_t = <|
   bb_label          : bir_label_t;
   bb_mc_tags        : bir_mc_tags_t option;
   bb_statements     : 'a list;
-  bb_last_statement : bir_stmt_end_t |>`;
+  bb_last_statement : 'ext_state_t bir_stmt_end_t |>`;
 
 val _ = Datatype `bir_ext_block_t = <|
   beb_label          : bir_label_t;
   (* TODO: If this relation also has the BIR program on LHS, we can model block-relative jumps (i.e. "next block") *)
-  beb_relation     : ((bir_state_t # (bir_state_t -> bool) # 'ext_state_t) -> (bir_state_t # 'ext_state_t) -> bool) |>`;
+  beb_relation     : 'ext_state_t beb_relation_t |>`;
 
 val _ = Datatype `bir_generic_block_t =
-  | BBlock_Stmts ('a bir_generic_stmt_block_t)
+  | BBlock_Stmts (('a,'ext_state_t)  bir_generic_stmt_block_t)
   | BBlock_Ext ('ext_state_t bir_ext_block_t)`;
 
 Datatype:
   bir_generic_program_t = BirProgram ((('a, 'ext_state_t) bir_generic_block_t) list)
 End
 
-Type bir_block_t = `` :(bir_stmt_basic_t, 'ext_state_t) bir_generic_block_t``
-Type bmc_block_t = `` :(bmc_stmt_basic_t, 'ext_state_t) bir_generic_block_t``
+Type bir_block_t = `` :('ext_state_t bir_stmt_basic_t, 'ext_state_t) bir_generic_block_t``
+Type bmc_block_t = `` :('ext_state_t bmc_stmt_basic_t, 'ext_state_t) bir_generic_block_t``
 
-Type bir_program_t = ``:(bir_stmt_basic_t, 'ext_state_t) bir_generic_program_t``
-Type bmc_program_t = ``:(bmc_stmt_basic_t, 'ext_state_t) bir_generic_program_t``
-
-val remove_inflight_def = Define`
-remove_inflight t l =
-    FILTER (\bi . case bi of BirInflight t0 _ => (t <> t0)) l
-`;
-
-val fresh_def = Define`
-fresh s = STRCAT "t" (n2s s.bst_counter)
-`;
+Type bir_program_t = ``:('ext_state_t bir_stmt_basic_t, 'ext_state_t) bir_generic_program_t``
+Type bmc_program_t = ``:('ext_state_t bmc_stmt_basic_t, 'ext_state_t) bir_generic_program_t``
 
 val bir_state_t_component_equality = DB.fetch "-" "bir_state_t_component_equality";
 val bir_programcounter_t_component_equality = DB.fetch "-" "bir_programcounter_t_component_equality";
+
+(*
+TODO
 val bir_state_ss = rewrites (type_rws ``:bir_state_t``);
 val bir_status_ss = rewrites (type_rws ``:bir_status_t``);
 
-val bir_stmt_ss = rewrites ((type_rws ``:bir_stmt_t``) @ (type_rws ``:bir_stmt_end_t``) @
-                            (type_rws ``:bir_stmt_basic_t``));
-
+val bir_stmt_ss = rewrites ((type_rws ``:'ext_state_t bir_stmt_t``)
+                    @ (type_rws ``:'ext_state_t bir_stmt_end_t``)
+                    @ (type_rws ``:'ext_state_t bir_stmt_basic_t``));
+*)
 
 (* ------------------------------------------------------------------------- *)
 (* Programs                                                                  *)
@@ -220,18 +217,25 @@ Cases_on `bir_get_program_block_info_by_label (BirProgram p) l` >| [
 (*  Program Counter                                                          *)
 (* ------------------------------------------------------------------------- *)
 
+Datatype:
+  bir_stmt_kind_t =
+    | BSGen (('a,'ext_state_t) bir_generic_stmt_t)
+    | BSExt ('ext_state_t beb_relation_t)
+End
+
 val bir_get_current_statement_def = Define `bir_get_current_statement p pc =
   option_CASE (bir_get_program_block_info_by_label p pc.bpc_label) NONE
     (\ (_, bl).
       case bl of
       | BBlock_Stmts stmts_bl =>
         if (pc.bpc_index < LENGTH stmts_bl.bb_statements)
-        then SOME (BStmtB (EL (pc.bpc_index) stmts_bl.bb_statements))
-        else (if pc.bpc_index = LENGTH stmts_bl.bb_statements then SOME (BStmtE stmts_bl.bb_last_statement) else NONE)
-      | BBlock_Ext ext_bl => NONE)`;
+        then SOME (BSGen $ BStmtB (EL (pc.bpc_index) stmts_bl.bb_statements))
+        else if pc.bpc_index = LENGTH stmts_bl.bb_statements
+          then SOME $ BSGen $ BStmtE stmts_bl.bb_last_statement else NONE
+      | BBlock_Ext ext_bl => SOME $ BSExt ext_bl.beb_relation )`;
 
 Definition bir_get_current_block_def:
-  bir_get_current_block p pc = 
+  bir_get_current_block p pc =
   option_CASE (bir_get_program_block_info_by_label p pc.bpc_label) NONE
     (\ (_, bl). SOME bl)
 End
@@ -271,31 +275,37 @@ val bir_state_set_failed_def = Define `bir_state_set_failed st =
 (*  Semantics of statements                                                  *)
 (* ------------------------------------------------------------------------- *)
 
-val bir_exec_stmt_assign_def = Define `bir_exec_stmt_assign ext_map v ex (st:bir_state_t, ext_st) =
-   case bir_eval_exp ext_map ex st.bst_environ ext_st of
+Definition bir_exec_stmt_assign_def:
+  bir_exec_stmt_assign v ex (st:bir_state_t, ext_st:'ext_state_t) =
+   case bir_eval_exp ex st.bst_environ ext_st of
      | SOME va => (case bir_env_write v va st.bst_environ of
                      | SOME env => (st with bst_environ := env)
                      | NONE => bir_state_set_typeerror st
                   )
-     | NONE => bir_state_set_typeerror st`;
+     | NONE => bir_state_set_typeerror st
+End
 
-val bir_exec_stmt_assert_def = Define `bir_exec_stmt_assert ext_map ex (st:bir_state_t, ext_st) =
-  case (option_CASE (bir_eval_exp ext_map ex st.bst_environ ext_st) NONE bir_dest_bool_val) of
+Definition bir_exec_stmt_assert_def:
+  bir_exec_stmt_assert ex (st:bir_state_t, ext_st :'ext_state_t) =
+  case (option_CASE (bir_eval_exp ex st.bst_environ ext_st) NONE bir_dest_bool_val) of
     | SOME T => st
     | SOME F => (st with bst_status := BST_AssertionViolated)
-    | NONE => bir_state_set_typeerror st`
+    | NONE => bir_state_set_typeerror st
+End
 
-val bir_exec_stmt_assume_def = Define `bir_exec_stmt_assume ext_map ex (st:bir_state_t, ext_st) =
-  case (option_CASE (bir_eval_exp ext_map ex st.bst_environ ext_st) NONE bir_dest_bool_val) of
+Definition bir_exec_stmt_assume_def:
+  bir_exec_stmt_assume ex (st:bir_state_t, ext_st : 'ext_state_t) =
+  case (option_CASE (bir_eval_exp ex st.bst_environ ext_st) NONE bir_dest_bool_val) of
     | SOME T => st
     | SOME F => (st with bst_status := BST_AssumptionViolated)
-    | NONE => bir_state_set_typeerror st`;
+    | NONE => bir_state_set_typeerror st
+End
 
 (*
-val bir_exec_stmt_ext_put_def = Define `bir_exec_stmt_ext_put ext_map (ext_name:string) ex (st:bir_state_t, ext_st:'ext_state_t) =
-  case bir_eval_exp ext_map ex st.bst_environ ext_st of
+val bir_exec_stmt_ext_put_def = Define `bir_exec_stmt_ext_put (ext_name:string) ex (st:bir_state_t, ext_st:'ext_state_t) =
+  case bir_eval_exp ex st.bst_environ ext_st of
     | SOME va =>
-     (case bir_lookup_put ext_map ext_name of
+     (case bir_lookup_put ext_name of
       | SOME f =>
        (case f va ext_st of
          | SOME ext_st' => (st, ext_st')
@@ -307,26 +317,26 @@ val bir_exec_stmt_ext_put_def = Define `bir_exec_stmt_ext_put ext_map (ext_name:
 *)
 
 val bir_exec_stmtB_def = Define `
-  (bir_exec_stmtB ext_map (BStmt_Assert ex) (st, ext_st:'ext_state_t) = (bir_exec_stmt_assert ext_map ex (st, ext_st), ext_st)) /\
-  (bir_exec_stmtB ext_map (BStmt_Assume ex) (st, ext_st) = (bir_exec_stmt_assume ext_map ex (st, ext_st), ext_st)) /\
-  (bir_exec_stmtB ext_map (BStmt_Assign v ex) (st, ext_st) = (bir_exec_stmt_assign ext_map v ex (st, ext_st), ext_st)) (*/\
-  (bir_exec_stmtB ext_map (BStmt_ExtPut ext_name ex) (st, ext_st) = bir_exec_stmt_ext_put ext_map ext_name ex (st, ext_st))*)`;
+  (bir_exec_stmtB (BStmt_Assert ex) (st: bir_state_t, ext_st:'ext_state_t) = (bir_exec_stmt_assert ex (st, ext_st), ext_st)) /\
+  (bir_exec_stmtB (BStmt_Assume ex) (st, ext_st) = (bir_exec_stmt_assume ex (st, ext_st), ext_st)) /\
+  (bir_exec_stmtB (BStmt_Assign v ex) (st, ext_st) = (bir_exec_stmt_assign v ex (st, ext_st), ext_st)) (*/\
+  (bir_exec_stmtB (BStmt_ExtPut ext_name ex) (st, ext_st) = bir_exec_stmt_ext_put ext_name ex (st, ext_st))*)`;
 
 val bir_exec_stmtB_exists =
   store_thm("bir_exec_stmtB_exists",
-  ``!ext_map h st ext_st:'ext_state_t.
+  ``!h st ext_st:'ext_state_t.
       ?st' ext_st'.
-        bir_exec_stmtB ext_map h (st, ext_st) = (st', ext_st')``,
+        bir_exec_stmtB h (st, ext_st) = (st', ext_st')``,
 
 Cases_on `h` >> (
   rpt strip_tac >>
   fs [bir_exec_stmtB_def]
 )(* >>
 fs [bir_exec_stmt_ext_put_def] >>
-Cases_on `bir_eval_exp ext_map b st.bst_environ ext_st` >> (
+Cases_on `bir_eval_exp b st.bst_environ ext_st` >> (
   fs []
 ) >>
-Cases_on `bir_lookup_put ext_map s` >> (
+Cases_on `bir_lookup_put s` >> (
   fs []
 ) >>
 Cases_on `x' x ext_st` >> (
@@ -334,8 +344,8 @@ Cases_on `x' x ext_st` >> (
 ) *)
 );
 
-val bir_exec_stmt_halt_def = Define `bir_exec_stmt_halt ext_map ex (st, ext_st:'ext_state_t) =
-  case bir_eval_exp ext_map ex st.bst_environ ext_st of
+val bir_exec_stmt_halt_def = Define `bir_exec_stmt_halt ex (st:bir_state_t, ext_st:'ext_state_t) =
+  case bir_eval_exp ex st.bst_environ ext_st of
     | NONE => bir_state_set_typeerror st
     | SOME v => st with bst_status := BST_Halted v`;
 
@@ -345,46 +355,47 @@ val bir_exec_stmt_jmp_to_label_def = Define `bir_exec_stmt_jmp_to_label p l st =
     else (st with bst_status := (BST_JumpOutside l))`;
 
 val bir_eval_label_exp_def = Define `
-   (bir_eval_label_exp ext_map (BLE_Label l) env (ext_st:'ext_state_t) = SOME l) /\
-   (bir_eval_label_exp ext_map (BLE_Exp e) env ext_st = case bir_eval_exp ext_map e env ext_st of
+   (bir_eval_label_exp (BLE_Label l) env (ext_st:'ext_state_t) = SOME l) /\
+   (bir_eval_label_exp (BLE_Exp e) env ext_st = case bir_eval_exp e env ext_st of
       | SOME (BVal_Imm i) => SOME (BL_Address i)
       | _ => NONE
    )`;
 
-val bir_exec_stmt_jmp_def = Define `bir_exec_stmt_jmp ext_map p le (st, ext_st:'ext_state_t) =
-    case bir_eval_label_exp ext_map le st.bst_environ ext_st of
+val bir_exec_stmt_jmp_def = Define `bir_exec_stmt_jmp p le (st, ext_st:'ext_state_t) =
+    case bir_eval_label_exp le st.bst_environ ext_st of
       | NONE => bir_state_set_typeerror st
       | SOME l => bir_exec_stmt_jmp_to_label p l st`;
 
-val bir_exec_stmt_cjmp_def = Define `bir_exec_stmt_cjmp ext_map p ec l1 l2 (st, ext_st:'ext_state_t) =
+val bir_exec_stmt_cjmp_def = Define `bir_exec_stmt_cjmp p ec l1 l2 (st, ext_st:'ext_state_t) =
   let
-    vobc = option_CASE (bir_eval_exp ext_map ec st.bst_environ ext_st) NONE bir_dest_bool_val
+    vobc = option_CASE (bir_eval_exp ec st.bst_environ ext_st) NONE bir_dest_bool_val
   in
   case vobc of
-    | SOME T => bir_exec_stmt_jmp ext_map p l1 (st, ext_st)
-    | SOME F => bir_exec_stmt_jmp ext_map p l2 (st, ext_st)
+    | SOME T => bir_exec_stmt_jmp p l1 (st, ext_st)
+    | SOME F => bir_exec_stmt_jmp p l2 (st, ext_st)
     | NONE => bir_state_set_typeerror st`;
 
 
 val bir_exec_stmtE_def = Define `
-  (bir_exec_stmtE ext_map p (BStmt_Jmp l) (st, ext_st:'ext_state_t) = bir_exec_stmt_jmp ext_map p l (st, ext_st)) /\
-  (bir_exec_stmtE ext_map p (BStmt_CJmp e l1 l2) (st, ext_st) = bir_exec_stmt_cjmp ext_map p e l1 l2 (st, ext_st)) /\
-  (bir_exec_stmtE ext_map p (BStmt_Halt ex) (st, ext_st) = bir_exec_stmt_halt ext_map ex (st, ext_st))`;
+  (bir_exec_stmtE p (BStmt_Jmp l) (st, ext_st:'ext_state_t) = bir_exec_stmt_jmp p l (st, ext_st)) /\
+  (bir_exec_stmtE p (BStmt_CJmp e l1 l2) (st, ext_st) = bir_exec_stmt_cjmp p e l1 l2 (st, ext_st)) /\
+  (bir_exec_stmtE p (BStmt_Halt ex) (st, ext_st) = bir_exec_stmt_halt ex (st, ext_st))`;
 
 
 val bir_exec_stmt_def = Define `
-  (bir_exec_stmt ext_map p (BStmtB (bst:bir_stmt_basic_t)) (st, ext_st:'ext_state_t) =
-     let (st', ext_st') = bir_exec_stmtB ext_map bst (st, ext_st) in
+  (bir_exec_stmt p (BStmtB (bst:'ext_state_t bir_stmt_basic_t)) (st:bir_state_t, ext_st:'ext_state_t) =
+     let (st', ext_st') = bir_exec_stmtB bst (st, ext_st) in
      if bir_state_is_terminated st' then (st', ext_st') else (st' with bst_pc updated_by bir_pc_next, ext_st')) /\
-  (bir_exec_stmt ext_map p (BStmtE bst) (st, ext_st) = (bir_exec_stmtE ext_map p bst (st, ext_st), ext_st))`;
+  (bir_exec_stmt p (BStmtE bst) (st, ext_st) = (bir_exec_stmtE p bst (st, ext_st), ext_st))`;
 
 (* bmc_exec_block_ext is defined later, in the promising semantics *)
-Definition bir_exec_block_ext:
+Definition bir_exec_block_ext_def:
   bir_exec_block_ext ext_fun (st:bir_state_t, ext_st:'ext_state_t) =
     (CHOICE (ext_fun (st, EMPTY:bir_state_t -> bool, ext_st))):(bir_state_t # 'ext_state_t)
 End
 
-val bir_exec_step_def = Define `bir_exec_step ext_map p (state, ext_st:'ext_state_t) =
+Definition bir_exec_step_def:
+  bir_exec_step p (state : bir_state_t, ext_st:'ext_state_t) =
   if (bir_state_is_terminated state) then (state, ext_st) else
   case (bir_get_current_block p state.bst_pc) of
   | NONE => (bir_state_set_failed state, ext_st)
@@ -393,9 +404,10 @@ val bir_exec_step_def = Define `bir_exec_step ext_map p (state, ext_st:'ext_stat
      | BBlock_Stmts stmts_bl =>
        (case (bir_get_current_statement p state.bst_pc) of
         | NONE => (bir_state_set_failed state, ext_st)
-        | SOME stm => (bir_exec_stmt ext_map p stm (state, ext_st)))
+        | SOME $ BSGen stm => bir_exec_stmt p stm (state, ext_st)
+        | SOME $ BSExt rel => bir_exec_block_ext rel (state, ext_st))
      | BBlock_Ext ext_bl => bir_exec_block_ext ext_bl.beb_relation (state, ext_st))
-`;
+End
 
 
 (* ------------------------------------------------------------------------- *)
@@ -412,17 +424,17 @@ val bir_exec_step_def = Define `bir_exec_step ext_map p (state, ext_st:'ext_stat
 (******************************)
 
 val bir_exec_infinite_steps_fun_def = Define `
-  (bir_exec_infinite_steps_fun ext_map p (st, ext_st:'ext_state_t) n = FUNPOW (bir_exec_step ext_map p) n (st,ext_st))`;
+  (bir_exec_infinite_steps_fun p (st, ext_st:'ext_state_t) n = FUNPOW (bir_exec_step p) n (st,ext_st))`;
 
 
 val bir_exec_infinite_steps_fun_REWRS = store_thm ("bir_exec_infinite_steps_fun_REWRS",
-``(!ext_map p st ext_st. (bir_exec_infinite_steps_fun ext_map p (st, ext_st:'ext_state_t) 0 = (st, ext_st))) /\
-  (!ext_map p st ext_st n. (bir_exec_infinite_steps_fun ext_map p (st, ext_st:'ext_state_t) (SUC n) =
-     (bir_exec_infinite_steps_fun ext_map p (bir_exec_step ext_map p (st, ext_st)) n)))``,
+``(!p st ext_st. (bir_exec_infinite_steps_fun p (st, ext_st:'ext_state_t) 0 = (st, ext_st))) /\
+  (!p st ext_st n. (bir_exec_infinite_steps_fun p (st, ext_st:'ext_state_t) (SUC n) =
+     (bir_exec_infinite_steps_fun p (bir_exec_step p (st, ext_st)) n)))``,
 
 SIMP_TAC std_ss [bir_exec_infinite_steps_fun_def, arithmeticTheory.FUNPOW] >>
 rpt strip_tac >>
-Cases_on `(bir_exec_step ext_map p (st,ext_st))` >>
+Cases_on `(bir_exec_step p (st,ext_st))` >>
 fs[bir_exec_infinite_steps_fun_def]);
 
 
@@ -436,19 +448,19 @@ val bir_state_COUNT_PC_def = Define `bir_state_COUNT_PC (count_failing:bool, pc_
 
 (* How often was a PC with a certain property reached. *)
 val bir_exec_infinite_steps_fun_COUNT_PCs_def = Define
-  `(bir_exec_infinite_steps_fun_COUNT_PCs pc_cond ext_map p (st, ext_st:'ext_state_t) 0 = 0) /\
-   (bir_exec_infinite_steps_fun_COUNT_PCs pc_cond ext_map p (st, ext_st) (SUC n) =
-    let r = bir_exec_infinite_steps_fun_COUNT_PCs pc_cond ext_map p
-               (bir_exec_step ext_map p (st, ext_st)) n in
-    if (bir_state_COUNT_PC pc_cond (bir_exec_step ext_map p (st, ext_st))) then SUC r else r)`
+  `(bir_exec_infinite_steps_fun_COUNT_PCs pc_cond p (st, ext_st:'ext_state_t) 0 = 0) /\
+   (bir_exec_infinite_steps_fun_COUNT_PCs pc_cond p (st, ext_st) (SUC n) =
+    let r = bir_exec_infinite_steps_fun_COUNT_PCs pc_cond p
+               (bir_exec_step p (st, ext_st)) n in
+    if (bir_state_COUNT_PC pc_cond (bir_exec_step p (st, ext_st))) then SUC r else r)`
 
 
 
 (* After how many steps do we terminate ? *)
 val bir_exec_infinite_steps_COUNT_STEPS_def = Define `
-  bir_exec_infinite_steps_COUNT_STEPS pc_cond max_steps_opt ext_map p (st, ext_st:'ext_state_t) = (OLEAST i.
-     bir_state_is_terminated $ FST (bir_exec_infinite_steps_fun ext_map p (st, ext_st) i) \/
-     (max_steps_opt = SOME (bir_exec_infinite_steps_fun_COUNT_PCs pc_cond ext_map p (st, ext_st) i))
+  bir_exec_infinite_steps_COUNT_STEPS pc_cond max_steps_opt p (st, ext_st:'ext_state_t) = (OLEAST i.
+     bir_state_is_terminated $ FST (bir_exec_infinite_steps_fun p (st, ext_st) i) \/
+     (max_steps_opt = SOME (bir_exec_infinite_steps_fun_COUNT_PCs pc_cond p (st, ext_st) i))
 )`;
 
 
@@ -465,7 +477,7 @@ val _ = Datatype `bir_execution_result_t =
 
     (* The execution does not terminate. Since the programs are finite, this means
        it loops. Therefore there are no step counts and no final state. *)
-  | BER_Looping 
+  | BER_Looping
 `;
 
 val bir_execution_result_ss = rewrites (type_rws ``:'ext_state_t bir_execution_result_t``);
@@ -494,37 +506,37 @@ val valOf_BER_Ended_steps_def = Define `valOf_BER_Ended_steps (BER_Ended step_co
 (* Now real execution. This is a clear definition, which is not well suited for evalation
    though. More efficient versions are derived later. We compute the no of steps and
    then execute this number of steps, recomputing values multiple times. *)
-val bir_exec_steps_GEN_def = Define `bir_exec_steps_GEN pc_cond ext_map p (state, ext_st:'ext_state_t) max_steps_opt =
-  let step_no = bir_exec_infinite_steps_COUNT_STEPS pc_cond max_steps_opt ext_map p (state, ext_st) in
+val bir_exec_steps_GEN_def = Define `bir_exec_steps_GEN pc_cond p (state, ext_st:'ext_state_t) max_steps_opt =
+  let step_no = bir_exec_infinite_steps_COUNT_STEPS pc_cond max_steps_opt p (state, ext_st) in
   (case step_no of
     | NONE => BER_Looping
     | SOME i => BER_Ended i
-                (bir_exec_infinite_steps_fun_COUNT_PCs pc_cond ext_map p (state, ext_st) i)
-                (bir_exec_infinite_steps_fun ext_map p (state, ext_st) i))`;
+                (bir_exec_infinite_steps_fun_COUNT_PCs pc_cond p (state, ext_st) i)
+                (bir_exec_infinite_steps_fun p (state, ext_st) i))`;
 
 
 (* A simple instance that just runs till termination. *)
 val bir_exec_steps_def = Define `
-  (bir_exec_steps ext_map p (state, ext_st:'ext_state_t) = bir_exec_steps_GEN (T, (\_. T)) ext_map p (state, ext_st) NONE)`;
+  (bir_exec_steps p (state, ext_st:'ext_state_t) = bir_exec_steps_GEN (T, (\_. T)) p (state, ext_st) NONE)`;
 
 (* A simple instance that counts all steps and has a fixed no of steps given.
    We are sure it terminates, therefore, the result is converted to a tuple. *)
 val bir_exec_step_n_def = Define `
-  bir_exec_step_n ext_map p (state, ext_st:'ext_state_t) n =
-  valOf_BER_Ended_steps (bir_exec_steps_GEN (T, (\_. T)) ext_map p (state, ext_st) (SOME n))`
+  bir_exec_step_n p (state, ext_st:'ext_state_t) n =
+  valOf_BER_Ended_steps (bir_exec_steps_GEN (T, (\_. T)) p (state, ext_st) (SOME n))`
 
 (* We might be interested in executing a certain no of blocks. *)
 val bir_exec_block_n_def = Define `
-  bir_exec_block_n ext_map p (state, ext_st:'ext_state_t) n =
-  valOf_BER_Ended (bir_exec_steps_GEN (F, (\pc. pc.bpc_index = 0)) ext_map p (state, ext_st) (SOME n))`
+  bir_exec_block_n p (state, ext_st:'ext_state_t) n =
+  valOf_BER_Ended (bir_exec_steps_GEN (F, (\pc. pc.bpc_index = 0)) p (state, ext_st) (SOME n))`
 
 (* Executing till a certain set of labels is useful as well. Since we might loop
    outside this set of labels, infinite runs are possible. *)
 val bir_exec_to_labels_n_def = Define `
-  bir_exec_to_labels_n ls ext_map p (state, ext_st:'ext_state_t) n =
-  bir_exec_steps_GEN (F, \pc. (pc.bpc_index = 0) /\ (pc.bpc_label IN ls)) ext_map p (state, ext_st) (SOME n)`
+  bir_exec_to_labels_n ls p (state, ext_st:'ext_state_t) n =
+  bir_exec_steps_GEN (F, \pc. (pc.bpc_index = 0) /\ (pc.bpc_label IN ls)) p (state, ext_st) (SOME n)`
 
 val bir_exec_to_labels_def = Define `
-  bir_exec_to_labels ls ext_map p (state, ext_st:'ext_state_t) = bir_exec_to_labels_n ls ext_map p (state, ext_st) 1`
+  bir_exec_to_labels ls p (state, ext_st:'ext_state_t) = bir_exec_to_labels_n ls p (state, ext_st) 1`
 
 val _ = export_theory();
